{-# OPTIONS --warn=noUserWarning #-}
module BoundedQuantification where

open import Level
open import ExtendedHierarchy renaming (_â‰¤_ to _â‰¤â‚’_; _<_ to _<â‚’_; _>_ to _>â‚’_)

--! BQ >

private variable
  â„“ â„“â€² â„“â‚ â„“â‚‚ â„“â‚ƒ â„“â‚„ : Level
  Î› Î›â€² Î›â‚ Î›â‚‚ Î›â‚ƒ Î›â‚„ : Level

-- Ordering on Levels ---------------------------------------------------------

-- axiom

--! LevelLe
data _â‰¤_ : Level â†’ Level â†’ Set where
  â‰¤-id   : âˆ€ â„“            â†’ â„“ â‰¤ â„“
  â‰¤-suc  : â„“ â‰¤ â„“â‚‚         â†’ â„“ â‰¤ suc â„“â‚‚
  â‰¤-lub  : âˆ€ â„“â‚ â†’ â„“ â‰¤ â„“â‚‚  â†’ â„“ â‰¤ (â„“â‚ âŠ” â„“â‚‚) 
  â‰¤-add  : âˆ€ â„“â‚ â†’ â„“ â‰¤ â„“â‚‚  â†’ â„“ â‰¤ Ï‰^ â„“â‚ + â„“â‚‚ 
  â‰¤-exp  : âˆ€ â„“â‚‚ â†’ â„“ â‰¤ â„“â‚  â†’ â„“ â‰¤ Ï‰^ â„“â‚ + â„“â‚‚ 

-- the important thing is, that the left hand side of the inequalities does not 
-- differ to the ones in the hypotheses, 
-- such that we can recurse in the BoundedLift / bounded-lift / bounded-unlift functions 

--! LevelLt
_<_ : Level â†’ Level â†’ Set
_<_ â„“â‚ â„“â‚‚ = suc â„“â‚ â‰¤ â„“â‚‚ 

--! Lim
data Lim : Level â†’ Set where
  lim  : âˆ€ {â„“}  â†’ zero < â„“  â†’ Lim (Ï‰^ â„“ + zero)
  add  : âˆ€ â„“â‚   â†’ Lim â„“â‚‚    â†’ Lim (Ï‰^ â„“â‚ + â„“â‚‚)
  
postulate 
--! AxiomsLe
  â‰¤-lublub   : â„“â‚ â‰¤ â„“â‚ƒ â†’ â„“â‚‚ â‰¤ â„“â‚ƒ â†’ (â„“â‚ âŠ” â„“â‚‚) â‰¤ â„“â‚ƒ
  <-suc-lim  : âˆ€ â„“â‚ â„“â‚‚ â†’ â„“â‚ < â„“â‚‚ â†’ Lim â„“â‚‚ â†’ suc â„“â‚ < â„“â‚‚

  -- unification fails
  -- no injectivity of suc / Ï‰^_+_ on postulates!
  -- proven on MutualOrd representation below
  -- propose to add injectivity? does this lead to inconsistency?

-- Bounded Quantification -----------------------------------------------------
--! BoundedLevel
record BoundedLevel (Î› : Level) : Set where
  constructor _,_  
  field  #_ : Level ;  #<Î› : #_ < Î›

open BoundedLevel public

bound : BoundedLevel Î› â†’ Level
bound {Î›} _ = Î›

-- Lifiting using Ordering ----------------------------------------------------

--! BoundedLift
BoundedLift  : â„“ â‰¤ Î› â†’ Set â„“ â†’ Set Î›
BoundedLift (â‰¤-id â„“)                  A = Lift â„“ A
BoundedLift (â‰¤-suc {â„“â‚‚ = â„“â‚‚} â„“â‰¤Î›)     A = Lift (suc â„“â‚‚) (BoundedLift â„“â‰¤Î› A)
BoundedLift (â‰¤-lub â„“â‚‚ â„“â‰¤Î›)            A = Lift â„“â‚‚ (BoundedLift â„“â‰¤Î› A)
BoundedLift (â‰¤-add {â„“â‚‚ = â„“â‚‚} â„“â‚ â„“â‰¤Î›)  A = cast (subsumption {â„“â‚ = â„“â‚‚} (add â„“â‚ id)) (Lift (Ï‰^ â„“â‚ + â„“â‚‚) (BoundedLift â„“â‰¤Î› A))
BoundedLift (â‰¤-exp {â„“â‚ = â„“â‚} â„“â‚‚ â„“â‰¤Î›)  A = cast (subsumption {â„“â‚ = â„“â‚} (exp â„“â‚‚ id)) (Lift (Ï‰^ â„“â‚ + â„“â‚‚) (BoundedLift â„“â‰¤Î› A))

bounded-lift : âˆ€ (â„“â‰¤Î› : â„“ â‰¤ Î›) â†’ {A : Set â„“} â†’ A â†’ BoundedLift â„“â‰¤Î› A
bounded-lift (â‰¤-id â„“)      a = lift a
bounded-lift (â‰¤-suc â„“â‰¤Î›)   a = lift (bounded-lift â„“â‰¤Î› a)
bounded-lift (â‰¤-lub _ â„“â‰¤Î›) a = lift (bounded-lift â„“â‰¤Î› a)
bounded-lift (â‰¤-add _ â„“â‰¤Î›) a = cast-intro _ (lift (bounded-lift â„“â‰¤Î› a))
bounded-lift (â‰¤-exp _ â„“â‰¤Î›) a = cast-intro _ (lift (bounded-lift â„“â‰¤Î› a))

bounded-unlift : âˆ€ (â„“â‰¤Î› : â„“ â‰¤ Î›) â†’ {A : Set â„“} â†’ BoundedLift â„“â‰¤Î› A â†’ A
bounded-unlift (â‰¤-id â„“)      (Level.lift a) = a
bounded-unlift (â‰¤-suc â„“â‰¤Î›)   (Level.lift a) = bounded-unlift â„“â‰¤Î› a
bounded-unlift (â‰¤-lub _ â„“â‰¤Î›) (Level.lift a) = bounded-unlift â„“â‰¤Î› a
bounded-unlift (â‰¤-add {â„“â‚‚ = â„“â‚‚} â„“â‚ â„“â‰¤Î›) {A = A} a with cast-elim _ {A = Lift (Ï‰^ â„“â‚ + â„“â‚‚) (BoundedLift â„“â‰¤Î› A)} a
... | lift a = bounded-unlift â„“â‰¤Î› a 
bounded-unlift (â‰¤-exp {â„“â‚ = â„“â‚} â„“â‚‚ â„“â‰¤Î›) {A = A} a with cast-elim _ {A = Lift (Ï‰^ â„“â‚ + â„“â‚‚) (BoundedLift â„“â‰¤Î› A)} a
... | lift a = bounded-unlift â„“â‰¤Î› a 

-- Properties for Lifiting using Ordering -------------------------------------

open import Relation.Binary.PropositionalEquality using (_â‰¡_; refl; sym; cong; trans; subst)
open import Data.Sum using (_âŠ_; injâ‚; injâ‚‚)
open import Data.Empty using (âŠ¥; âŠ¥-elim)

module Properties where  
  unlift-lift-cancel : âˆ€ (â„“â‰¤Î› : â„“ â‰¤ Î›) {A : Set â„“} â†’ (a : A) â†’ 
    bounded-unlift â„“â‰¤Î› (bounded-lift â„“â‰¤Î› a) â‰¡ a 
  unlift-lift-cancel (â‰¤-id â„“)      a = refl  
  unlift-lift-cancel (â‰¤-suc â„“â‰¤Î›)   a = unlift-lift-cancel â„“â‰¤Î› a
  unlift-lift-cancel (â‰¤-lub _ â„“â‰¤Î›) a = unlift-lift-cancel â„“â‰¤Î› a
  unlift-lift-cancel (â‰¤-add {â„“â‚‚ = â„“â‚‚} â„“â‚ â„“â‰¤Î›) a 
    rewrite cast-elim-intro-cancel (subsumption {â„“â‚ = â„“â‚‚} (add â„“â‚ id)) (lift {â„“ = Ï‰^ â„“â‚ + â„“â‚‚} (bounded-lift â„“â‰¤Î› a))
    = unlift-lift-cancel â„“â‰¤Î› a 
  unlift-lift-cancel (â‰¤-exp {â„“â‚ = â„“â‚} â„“â‚‚ â„“â‰¤Î›) a 
    rewrite cast-elim-intro-cancel (subsumption {â„“â‚ = â„“â‚} (exp â„“â‚‚ id)) (lift {â„“ = Ï‰^ â„“â‚ + â„“â‚‚} (bounded-lift â„“â‰¤Î› a))
    = unlift-lift-cancel â„“â‰¤Î› a

-- Proving the postulates on the MutualOrd Representation ---------------------

â‰¤-idâ€² : âˆ€ a â†’ a â‰¤â‚’ a
â‰¤-idâ€² a = injâ‚‚ refl

<-sucâ€² : âˆ€ a b â†’ a <â‚’ b â†’ a <â‚’ sucâ‚’ b
<-sucâ€² a b <â‚ = <â‚
<-sucâ€² a b (<â‚‚ a<b) = <â‚‚ a<b
<-sucâ€² a b (<â‚ƒ refl a<b) = <â‚ƒ refl (<-sucâ€² _ _ a<b)

â‰¤-sucâ€² : âˆ€ a b â†’ a â‰¤â‚’ b â†’ a â‰¤â‚’ sucâ‚’ b
â‰¤-sucâ€² a b (injâ‚ x) = injâ‚ (<-sucâ€² a b x)
â‰¤-sucâ€² a b (injâ‚‚ refl) = injâ‚ (a<suc[a] _)
  where a<suc[a] : âˆ€ a â†’ a <â‚’ sucâ‚’ a 
        a<suc[a] ğŸ = <â‚
        a<suc[a] Ï‰^ a + aâ‚ [ x ] = <â‚ƒ refl (a<suc[a] _)
        
<-lubâ€² : âˆ€ a b c â†’ a <â‚’ b â†’ a <â‚’ (b âŠ”â‚’ c)
<-lubâ€² a b ğŸ a<b = subst (_ <â‚’_) (sym (right-idâ€² _)) a<b
<-lubâ€² a Ï‰^ ba + bb [ br ] Ï‰^ ca + cb [ cr ] a<b with <-tri ba ca
... | injâ‚ x = <-trans a<b (<â‚‚ x)
... | injâ‚‚ (injâ‚ x) = a<b
... | injâ‚‚ (injâ‚‚ refl) with <-tri bb cb 
... | injâ‚ x = <-trans a<b (<â‚ƒ refl x)
... | injâ‚‚ (injâ‚ x) = a<b
... | injâ‚‚ (injâ‚‚ refl) = subst (a <â‚’_) (MutualOrdâ¼ refl refl) a<b 

â‰¤-lubâ€² :  âˆ€ a b c â†’ a â‰¤â‚’ b â†’ a â‰¤â‚’ (b âŠ”â‚’ c)
â‰¤-lubâ€² a b c (injâ‚ x) = injâ‚ (<-lubâ€² _ _ _ x)
â‰¤-lubâ€² a b ğŸ (injâ‚‚ refl) = injâ‚‚ (right-idâ€² a)
â‰¤-lubâ€² ğŸ b Ï‰^ c + câ‚ [ x ] (injâ‚‚ refl) = injâ‚ <â‚
â‰¤-lubâ€² Ï‰^ aa + ab [ ar ] b Ï‰^ ca + cb [ cr ] (injâ‚‚ refl) with <-tri aa ca 
... | injâ‚ x = injâ‚ (<â‚‚ x)
... | injâ‚‚ (injâ‚ x) = injâ‚‚ refl
... | injâ‚‚ (injâ‚‚ refl) with <-tri ab cb
... | injâ‚ x = injâ‚ (<â‚ƒ refl x)
... | injâ‚‚ (injâ‚ x) = injâ‚‚ refl
... | injâ‚‚ (injâ‚‚ refl) = injâ‚‚ (MutualOrdâ¼ refl refl)

â‰¤-addâ€²  : âˆ€ a b r â†’ a â‰¤â‚’ b â†’ a â‰¤â‚’ Ï‰^ a + b [ r ]
â‰¤-addâ€² a b r aâ‰¤b = injâ‚ (fst< _ _ _) 

â‰¤-expâ€²  : âˆ€ a b r â†’ a â‰¤â‚’ b â†’ a â‰¤â‚’ Ï‰^ b + a [ r ]
â‰¤-expâ€² a b r aâ‰¤b = injâ‚ (rest< _ _ _) 

data _â‰¤â‚’â€²_ : MutualOrd â†’ MutualOrd â†’ Set where
  â‰¤â‚’â€²-id   : âˆ€ a                 â†’ a â‰¤â‚’â€² a
  â‰¤â‚’â€²-suc  : âˆ€ a b     â†’ a â‰¤â‚’â€² b â†’ a â‰¤â‚’â€² sucâ‚’ b
  â‰¤â‚’â€²-lub  : âˆ€ a b c   â†’ a â‰¤â‚’â€² b â†’ a â‰¤â‚’â€² (b âŠ”â‚’ c) 
  â‰¤â‚’â€²-add  : âˆ€ a b c r â†’ a â‰¤â‚’â€² c â†’ a â‰¤â‚’â€² Ï‰^ b + c [ r ] 
  â‰¤â‚’â€²-exp  : âˆ€ a b c r â†’ a â‰¤â‚’â€² b â†’ a â‰¤â‚’â€² Ï‰^ b + c [ r ]

-- completeness : âˆ€ a b â†’ a â‰¤â‚’ b â†’ a â‰¤â‚’â€² b  
-- completeness a b (injâ‚ <â‚) = {!   !}
-- completeness Ï‰^ aa + ab [ ar ] Ï‰^ ba + bb [ br ] (injâ‚ (<â‚‚ x)) = lemma _ _ _ _ _ _ (completeness _ _ (injâ‚ x))
--   where lemma : âˆ€ a b c d r s â†’ a â‰¤â‚’â€² c â†’ Ï‰^ a + b [ r ] â‰¤â‚’â€² Ï‰^ c + d [ s ]
--         lemma a _ _ _ _ _ (â‰¤â‚’â€²-id .a) = {!   !}
--         lemma a _ _ _ _ _ (â‰¤â‚’â€²-suc .a b x) = {!   !}
--         lemma a _ _ _ _ _ (â‰¤â‚’â€²-lub .a b c x) = {!   !}
--         lemma a _ _ _ _ _ (â‰¤â‚’â€²-add .a b c r x) = {!   !}
--         lemma a _ _ _ _ _ (â‰¤â‚’â€²-exp .a b c r x) = {!   !}
-- completeness a b (injâ‚ (<â‚ƒ x xâ‚)) = {!   !}
-- completeness a b (injâ‚‚ refl) = â‰¤â‚’â€²-id _

data LimOrd : MutualOrd â†’ Set where 
  limâ€² : âˆ€ a â†’ a >â‚’ ğŸ â†’ LimOrd (Ï‰^âŸ¨ a âŸ©)
  addâ€² : âˆ€ a b r â†’ LimOrd b â†’ LimOrd Ï‰^ a + b [ r ]

LimOrd[a]â†’fst[a]>ğŸ : âˆ€ a â†’ LimOrd a â†’ fst a >â‚’ ğŸ
LimOrd[a]â†’fst[a]>ğŸ _ (limâ€² _ x)                  = x
LimOrd[a]â†’fst[a]>ğŸ _ (addâ€² _ _ (injâ‚ x) lima)    = <-trans (LimOrd[a]â†’fst[a]>ğŸ _ lima) x
LimOrd[a]â†’fst[a]>ğŸ _ (addâ€² _ _ (injâ‚‚ refl) lima) = LimOrd[a]â†’fst[a]>ğŸ _ lima

<-suc-limâ€² : âˆ€ a b â†’ a <â‚’ b â†’ LimOrd b â†’ sucâ‚’ a <â‚’ b
<-suc-limâ€² a b <â‚ limb = <â‚‚ (LimOrd[a]â†’fst[a]>ğŸ _ limb)
<-suc-limâ€² a b (<â‚‚ a<b) limb = <â‚‚ a<b
<-suc-limâ€² a b (<â‚ƒ refl a<b) (addâ€² _ _ _ limb) = <â‚ƒ refl (<-suc-limâ€² _ _ a<b limb) 

<-lublubâ€² : âˆ€ a b c â†’ a <â‚’ c â†’ b <â‚’ c â†’ (a âŠ”â‚’ b) <â‚’ c
<-lublubâ€² a b c <â‚ b<c = b<c
<-lublubâ€² a b c a<c <â‚ = subst (_<â‚’ _) (sym (right-idâ€²  _)) a<c
<-lublubâ€² Ï‰^ aa + ab [ r ] Ï‰^ ba + bb [ s ] Ï‰^ ca + cb [ t ] (<â‚‚ a<c) (<â‚‚ b<c) with <-tri aa ba
... | injâ‚ x = <â‚‚ b<c
... | injâ‚‚ (injâ‚ x) = <â‚‚ a<c
... | injâ‚‚ (injâ‚‚ refl) with <-tri ab bb
... | injâ‚ x = <â‚‚ b<c
... | injâ‚‚ (injâ‚ x) = <â‚‚ a<c
... | injâ‚‚ (injâ‚‚ refl) = <â‚‚ b<c
<-lublubâ€² Ï‰^ aa + ab [ r ] Ï‰^ ba + bb [ s ] Ï‰^ ca + cb [ t ] (<â‚‚ a<c) (<â‚ƒ refl b<c) with  <-tri aa ba
... | injâ‚ x = <â‚ƒ refl b<c
... | injâ‚‚ (injâ‚ x) = <â‚‚ a<c
... | injâ‚‚ (injâ‚‚ refl) with <-tri ab bb
... | injâ‚ x = <â‚ƒ refl b<c
... | injâ‚‚ (injâ‚ x) = âŠ¥-elim (<-irrefl a<c)
... | injâ‚‚ (injâ‚‚ refl) = <â‚ƒ refl b<c
<-lublubâ€² Ï‰^ aa + ab [ r ] Ï‰^ ba + bb [ s ] Ï‰^ ca + cb [ t ] (<â‚ƒ refl a<c) (<â‚‚ b<c) with <-tri aa ba
... | injâ‚ x = <â‚‚ b<c
... | injâ‚‚ (injâ‚ x) = <â‚ƒ refl a<c
... | injâ‚‚ (injâ‚‚ refl) with <-tri ab bb
... | injâ‚ x = âŠ¥-elim (<-irrefl b<c)
... | injâ‚‚ (injâ‚ x) = <â‚ƒ refl a<c
... | injâ‚‚ (injâ‚‚ refl) = âŠ¥-elim (<-irrefl b<c)
<-lublubâ€² Ï‰^ aa + ab [ r ] Ï‰^ ba + bb [ s ] Ï‰^ ca + cb [ t ] (<â‚ƒ refl a<c) (<â‚ƒ refl b<c) with <-tri aa aa
... | injâ‚ x = <â‚ƒ refl b<c
... | injâ‚‚ (injâ‚ x) = <â‚ƒ refl a<c
... | injâ‚‚ (injâ‚‚ refl) with <-tri ab bb
... | injâ‚ x = <â‚ƒ refl b<c
... | injâ‚‚ (injâ‚ x) = <â‚ƒ refl a<c
... | injâ‚‚ (injâ‚‚ refl) = <â‚ƒ refl b<c

â‰¤-lublubâ€² : âˆ€ a b c â†’ a â‰¤â‚’ c â†’ b â‰¤â‚’ c â†’ (a âŠ”â‚’ b) â‰¤â‚’ c
â‰¤-lublubâ€² a b c (injâ‚ x) (injâ‚ y) = injâ‚ (<-lublubâ€² _ _ _ x y) 
â‰¤-lublubâ€² a b c (injâ‚ x) (injâ‚‚ refl) = injâ‚‚ (sym (<-âŠ”â‚’-right _ _ x)) 
â‰¤-lublubâ€² a b c (injâ‚‚ refl) (injâ‚ x) = injâ‚‚ (sym (<-âŠ”â‚’-left _ _ x))       
â‰¤-lublubâ€² a b c (injâ‚‚ refl) (injâ‚‚ refl) rewrite idemâ€² a = injâ‚‚ refl 
 