{-# OPTIONS --allow-unsolved-metas #-}
module BoundQuantification where

open import Level
open import ExtendedHierarchy renaming (_â‰¤_ to _â‰¤áµ’_; _<_ to _<áµ’_; _>_ to _>áµ’_)

private variable
  â„“ â„“â€² â„“â‚ â„“â‚‚ â„“â‚ƒ â„“â‚„ : Level
  Î› Î›â€² Î›â‚ Î›â‚‚ Î›â‚ƒ Î›â‚„ : Level

-- Ordering on Levels ---------------------------------------------------------

-- axiom

data _â‰¤_ : Level â†’ Level â†’ Set where
  â‰¤-id  : âˆ€ â„“ â†’ â„“ â‰¤ â„“
  â‰¤-suc : â„“â‚ â‰¤ â„“â‚‚ â†’ â„“â‚ â‰¤ suc â„“â‚‚
  â‰¤-lub : âˆ€ â„“â‚‚ â†’ â„“ â‰¤ â„“â‚ â†’ â„“ â‰¤ (â„“â‚ âŠ” â„“â‚‚) 
  â‰¤-add : âˆ€ â„“â‚ â†’ â„“ â‰¤ â„“â‚‚ â†’ â„“ â‰¤ Ï‰^ â„“â‚ + â„“â‚‚ 
  â‰¤-exp : âˆ€ â„“â‚‚ â†’ â„“ â‰¤ â„“â‚ â†’ â„“ â‰¤ Ï‰^ â„“â‚ + â„“â‚‚ 

_<_ : Level â†’ Level â†’ Set
_<_ â„“â‚ â„“â‚‚ = suc â„“â‚ â‰¤ â„“â‚‚ 

-- the important thing is, that the left hand side of the inequalities does not 
-- differ to the ones in the hypotheses, 
-- such that we can recurse in the BoundLift / bound-lift / bound-unlift functions 

data Lim : Level â†’ Set where
  lim : âˆ€ â„“ â†’ zero < â„“ â†’ Lim (Ï‰^ â„“ + zero)
  add : âˆ€ â„“â‚ â„“â‚‚ â†’ Lim â„“â‚‚ â†’ Lim (Ï‰^ â„“â‚ + â„“â‚‚)
  
postulate 
  â‰¤-lublub  : â„“â‚ â‰¤ â„“â‚ƒ â†’ â„“â‚‚ â‰¤ â„“â‚ƒ â†’ (â„“â‚ âŠ” â„“â‚‚) â‰¤ â„“â‚ƒ
  <-suc-lim : âˆ€ â„“â‚ â„“â‚‚ â†’ â„“â‚ < â„“â‚‚ â†’ Lim â„“â‚‚ â†’ suc â„“â‚ < â„“â‚‚
  -- unification fails
  -- no injectivity of suc / Ï‰^_+_ on postulates!
  -- proven on MutualOrd representation below

-- Bounded Quantification -----------------------------------------------------
record BoundLevel (Î› : Level) : Set where
  constructor _,_  
  field 
    # : Level
    #<Î› : # < Î›

open BoundLevel public

bound : BoundLevel Î› â†’ Level
bound {Î›} _ = Î›

-- Lifiting using Ordering ----------------------------------------------------

BoundLift  : â„“ â‰¤ Î› â†’ Set â„“ â†’ Set Î›
BoundLift (â‰¤-id â„“)                 A = Lift â„“ A
BoundLift (â‰¤-suc {â„“â‚‚ = â„“â‚‚} â„“â‰¤Î›)    A = Lift (suc â„“â‚‚) (BoundLift â„“â‰¤Î› A)
BoundLift (â‰¤-lub â„“â‚‚ â„“â‰¤Î›)           A = Lift â„“â‚‚ (BoundLift â„“â‰¤Î› A)
BoundLift (â‰¤-add {â„“â‚‚ = â„“â‚‚} â„“â‚ â„“â‰¤Î›) A = cast (subsumption-addâ‚â‚€ {â„“ = â„“â‚‚} {â„“â‚ = â„“â‚}) (Lift (Ï‰^ â„“â‚ + â„“â‚‚) (BoundLift â„“â‰¤Î› A))
BoundLift (â‰¤-exp {â„“â‚ = â„“â‚} â„“â‚‚ â„“â‰¤Î›) A = cast (subsumption-expâ‚â‚€ {â„“ = â„“â‚} {â„“â‚ = â„“â‚‚}) (Lift (Ï‰^ â„“â‚ + â„“â‚‚) (BoundLift â„“â‰¤Î› A))

bound-lift : âˆ€ (â„“â‰¤Î› : â„“ â‰¤ Î›) â†’ {A : Set â„“} â†’ A â†’ BoundLift â„“â‰¤Î› A
bound-lift (â‰¤-id â„“)      a = lift a
bound-lift (â‰¤-suc â„“â‰¤Î›)   a = lift (bound-lift â„“â‰¤Î› a)
bound-lift (â‰¤-lub _ â„“â‰¤Î›) a = lift (bound-lift â„“â‰¤Î› a)
bound-lift (â‰¤-add _ â„“â‰¤Î›) a = cast-push _ (lift (bound-lift â„“â‰¤Î› a))
bound-lift (â‰¤-exp _ â„“â‰¤Î›) a = cast-push _ (lift (bound-lift â„“â‰¤Î› a))

bound-unlift : âˆ€ (â„“â‰¤Î› : â„“ â‰¤ Î›) â†’ {A : Set â„“} â†’ BoundLift â„“â‰¤Î› A â†’ A
bound-unlift (â‰¤-id â„“)      (Level.lift a) = a
bound-unlift (â‰¤-suc â„“â‰¤Î›)   (Level.lift a) = bound-unlift â„“â‰¤Î› a
bound-unlift (â‰¤-lub _ â„“â‰¤Î›) (Level.lift a) = bound-unlift â„“â‰¤Î› a
bound-unlift (â‰¤-add {â„“â‚‚ = â„“â‚‚} â„“â‚ â„“â‰¤Î›) {A = A} a with cast-pop _ {A = Lift (Ï‰^ â„“â‚ + â„“â‚‚) (BoundLift â„“â‰¤Î› A)} a
... | lift a = bound-unlift â„“â‰¤Î› a 
bound-unlift (â‰¤-exp {â„“â‚ = â„“â‚} â„“â‚‚ â„“â‰¤Î›) {A = A} a with cast-pop _ {A = Lift (Ï‰^ â„“â‚ + â„“â‚‚) (BoundLift â„“â‰¤Î› A)} a
... | lift a = bound-unlift â„“â‰¤Î› a 

-- Properties for Lifiting using Ordering -------------------------------------

open import Relation.Binary.PropositionalEquality using (_â‰¡_; refl; sym; cong; trans; subst)
open import Data.Sum using (_âŠ_; injâ‚; injâ‚‚)
open import Data.Empty using (âŠ¥; âŠ¥-elim)

module Properties where  
  unlift-lift-cancel : âˆ€ (â„“â‰¤Î› : â„“ â‰¤ Î›) {A : Set â„“} â†’ (a : A) â†’ 
    bound-unlift â„“â‰¤Î› (bound-lift â„“â‰¤Î› a) â‰¡ a 
  unlift-lift-cancel (â‰¤-id â„“)      a = refl  
  unlift-lift-cancel (â‰¤-suc â„“â‰¤Î›)   a = unlift-lift-cancel â„“â‰¤Î› a
  unlift-lift-cancel (â‰¤-lub _ â„“â‰¤Î›) a = unlift-lift-cancel â„“â‰¤Î› a
  unlift-lift-cancel (â‰¤-add {â„“â‚‚ = â„“â‚‚} â„“â‚ â„“â‰¤Î›) a 
    rewrite cast-pop-push-cancel (subsumption-addâ‚â‚€ {â„“ = â„“â‚‚} {â„“â‚ = â„“â‚}) (lift {â„“ = Ï‰^ â„“â‚ + â„“â‚‚} (bound-lift â„“â‰¤Î› a))
    = unlift-lift-cancel â„“â‰¤Î› a 
  unlift-lift-cancel (â‰¤-exp {â„“â‚ = â„“â‚} â„“â‚‚ â„“â‰¤Î›) a -- unlift-lift-cancel â„“â‰¤Î› a
    rewrite cast-pop-push-cancel (subsumption-expâ‚â‚€ {â„“ = â„“â‚} {â„“â‚ = â„“â‚‚}) (lift {â„“ = Ï‰^ â„“â‚ + â„“â‚‚} (bound-lift â„“â‰¤Î› a))
    = unlift-lift-cancel â„“â‰¤Î› a

  -- lift-unlift-cancel : âˆ€ (â„“â‰¤Î› : â„“ â‰¤ Î›) {A : Set â„“} â†’ (a : BoundLift â„“â‰¤Î› A) â†’ 
  --   bound-lift â„“â‰¤Î› (bound-unlift â„“â‰¤Î› a) â‰¡ a 
  -- lift-unlift-cancel (â‰¤-id â„“)      a        = refl             
  -- lift-unlift-cancel (â‰¤-suc â„“â‰¤Î›)   (lift a) = cong lift (lift-unlift-cancel â„“â‰¤Î› a)
  -- lift-unlift-cancel (â‰¤-lub _ â„“â‰¤Î›) (lift a) = cong lift (lift-unlift-cancel â„“â‰¤Î› a)
  -- lift-unlift-cancel (â‰¤-add {â„“â‚‚ = â„“â‚‚} â„“â‚ â„“â‰¤Î›) {A} a with lift-unlift-cancel â„“â‰¤Î› (lower (cast-pop _ {A = Lift (Ï‰^ â„“â‚ + â„“â‚‚) (BoundLift â„“â‰¤Î› A)} a))
  -- ... | ih = {! cong lift ih    !}
  -- lift-unlift-cancel (â‰¤-exp _ â„“â‰¤Î›) a  =  {!   !}

-- Proving the postulates on the MutualOrd Representation ---------------------

data LimOrd : MutualOrd â†’ Set where 
  limâ€² : âˆ€ a â†’ a >áµ’ ğŸ â†’ LimOrd (Ï‰^âŸ¨ a âŸ©)
  addâ€² : âˆ€ a b r â†’ LimOrd b â†’ LimOrd Ï‰^ a + b [ r ]

LimOrd[a]â†’fst[a]>ğŸ : âˆ€ a â†’ LimOrd a â†’ fst a >áµ’ ğŸ
LimOrd[a]â†’fst[a]>ğŸ _ (limâ€² _ x)                  = x
LimOrd[a]â†’fst[a]>ğŸ _ (addâ€² _ _ (injâ‚ x) lima)    = <-trans (LimOrd[a]â†’fst[a]>ğŸ _ lima) x
LimOrd[a]â†’fst[a]>ğŸ _ (addâ€² _ _ (injâ‚‚ refl) lima) = LimOrd[a]â†’fst[a]>ğŸ _ lima

<-suc-limâ€² : âˆ€ a b â†’ a <áµ’ b â†’ LimOrd b â†’ sucâ‚’ a <áµ’ b
<-suc-limâ€² a b <â‚ limb = <â‚‚ (LimOrd[a]â†’fst[a]>ğŸ _ limb)
<-suc-limâ€² a b (<â‚‚ a<b) limb = <â‚‚ a<b
<-suc-limâ€² a b (<â‚ƒ refl a<b) (addâ€² _ _ _ limb) = <â‚ƒ refl (<-suc-limâ€² _ _ a<b limb) 

âŠ”â‚’-idem : âˆ€ a â†’ (a âŠ”â‚’ a) â‰¡ a
âŠ”â‚’-idem ğŸ = refl
âŠ”â‚’-idem Ï‰^ a + b [ r ] with <-tri a a 
... | injâ‚ a<a = âŠ¥-elim (<-irrefl a<a)
... | injâ‚‚ (injâ‚ a<a) = âŠ¥-elim (<-irrefl a<a)
... | injâ‚‚ (injâ‚‚ refl) with <-tri b b 
... | injâ‚ a<a = âŠ¥-elim (<-irrefl a<a)
... | injâ‚‚ (injâ‚ a<a) = âŠ¥-elim (<-irrefl a<a)
... | injâ‚‚ (injâ‚‚ refl) = refl

right-id : âˆ€ a â†’ (a âŠ”â‚’ ğŸ) â‰¡ a
right-id ğŸ = refl
right-id Ï‰^ a + aâ‚ [ x ] = refl

âŠ”â‚’-<áµ’ : âˆ€ a b â†’ a <áµ’ b â†’ (a âŠ”â‚’ b) â‰¡ b
âŠ”â‚’-<áµ’ a b <â‚            = refl
âŠ”â‚’-<áµ’ Ï‰^ aa + ab [ r ] Ï‰^ ba + bb [ s ] (<â‚‚ x) with <-tri aa ba 
... | injâ‚ x = refl
... | injâ‚‚ (injâ‚ y) = âŠ¥-elim (Lm[â‰¥â†’Â¬<] (injâ‚ x) y)
... | injâ‚‚ (injâ‚‚ refl) with <-tri ab bb
... | injâ‚ x = refl
... | injâ‚‚ (injâ‚ y) = âŠ¥-elim (<-irrefl x)
... | injâ‚‚ (injâ‚‚ refl) = refl
âŠ”â‚’-<áµ’ Ï‰^ aa + ab [ r ] Ï‰^ ba + bb [ s ] (<â‚ƒ refl x) with <-tri ba ba 
... | injâ‚ x = refl
... | injâ‚‚ (injâ‚ x) = âŠ¥-elim (<-irrefl x)
... | injâ‚‚ (injâ‚‚ refl) with <-tri ab bb
... | injâ‚ x = refl
... | injâ‚‚ (injâ‚ y) = âŠ¥-elim (Lm[â‰¥â†’Â¬<] (injâ‚ x) y)
... | injâ‚‚ (injâ‚‚ refl) = refl

âŠ”â‚’-<áµ’â€² : âˆ€ a b â†’ b <áµ’ a â†’ (a âŠ”â‚’ b) â‰¡ a
âŠ”â‚’-<áµ’â€² a b <â‚            = refl
âŠ”â‚’-<áµ’â€² Ï‰^ aa + ab [ r ] Ï‰^ ba + bb [ s ] (<â‚‚ x) with <-tri aa ba 
... | injâ‚ y = âŠ¥-elim (Lm[â‰¥â†’Â¬<] (injâ‚ x) y)
... | injâ‚‚ (injâ‚ y) = refl 
... | injâ‚‚ (injâ‚‚ refl) with <-tri ab bb
... | injâ‚ y = âŠ¥-elim (<-irrefl x) 
... | injâ‚‚ (injâ‚ y) = âŠ¥-elim (<-irrefl x)
... | injâ‚‚ (injâ‚‚ refl) = MutualOrdâ¼ refl refl 
âŠ”â‚’-<áµ’â€² Ï‰^ aa + ab [ r ] Ï‰^ ba + bb [ s ] (<â‚ƒ refl x) with <-tri ba ba 
... | injâ‚ y = âŠ¥-elim (<-irrefl y)
... | injâ‚‚ (injâ‚ y) = refl 
... | injâ‚‚ (injâ‚‚ refl) with <-tri ab bb
... | injâ‚ y = âŠ¥-elim (Lm[â‰¥â†’Â¬<] (injâ‚ x) y)
... | injâ‚‚ (injâ‚ y) = refl
... | injâ‚‚ (injâ‚‚ refl) = MutualOrdâ¼ refl refl 

<-lublub : âˆ€ a b c â†’ a <áµ’ c â†’ b <áµ’ c â†’ (a âŠ”â‚’ b) <áµ’ c
<-lublub a b c <â‚ b<c = b<c
<-lublub a b c a<c <â‚ = subst (_<áµ’ _) (sym (right-id _)) a<c
<-lublub Ï‰^ aa + ab [ r ] Ï‰^ ba + bb [ s ] Ï‰^ ca + cb [ t ] (<â‚‚ a<c) (<â‚‚ b<c) with <-tri aa ba
... | injâ‚ x = <â‚‚ b<c
... | injâ‚‚ (injâ‚ x) = <â‚‚ a<c
... | injâ‚‚ (injâ‚‚ refl) with <-tri ab bb
... | injâ‚ x = <â‚‚ b<c
... | injâ‚‚ (injâ‚ x) = <â‚‚ a<c
... | injâ‚‚ (injâ‚‚ refl) = <â‚‚ b<c
<-lublub Ï‰^ aa + ab [ r ] Ï‰^ ba + bb [ s ] Ï‰^ ca + cb [ t ] (<â‚‚ a<c) (<â‚ƒ refl b<c) with  <-tri aa ba
... | injâ‚ x = <â‚ƒ refl b<c
... | injâ‚‚ (injâ‚ x) = <â‚‚ a<c
... | injâ‚‚ (injâ‚‚ refl) with <-tri ab bb
... | injâ‚ x = <â‚ƒ refl b<c
... | injâ‚‚ (injâ‚ x) = âŠ¥-elim (<-irrefl a<c)
... | injâ‚‚ (injâ‚‚ refl) = <â‚ƒ refl b<c
<-lublub Ï‰^ aa + ab [ r ] Ï‰^ ba + bb [ s ] Ï‰^ ca + cb [ t ] (<â‚ƒ refl a<c) (<â‚‚ b<c) with <-tri aa ba
... | injâ‚ x = <â‚‚ b<c
... | injâ‚‚ (injâ‚ x) = <â‚ƒ refl a<c
... | injâ‚‚ (injâ‚‚ refl) with <-tri ab bb
... | injâ‚ x = âŠ¥-elim (<-irrefl b<c)
... | injâ‚‚ (injâ‚ x) = <â‚ƒ refl a<c
... | injâ‚‚ (injâ‚‚ refl) = âŠ¥-elim (<-irrefl b<c)
<-lublub Ï‰^ aa + ab [ r ] Ï‰^ ba + bb [ s ] Ï‰^ ca + cb [ t ] (<â‚ƒ refl a<c) (<â‚ƒ refl b<c) with <-tri aa aa
... | injâ‚ x = <â‚ƒ refl b<c
... | injâ‚‚ (injâ‚ x) = <â‚ƒ refl a<c
... | injâ‚‚ (injâ‚‚ refl) with <-tri ab bb
... | injâ‚ x = <â‚ƒ refl b<c
... | injâ‚‚ (injâ‚ x) = <â‚ƒ refl a<c
... | injâ‚‚ (injâ‚‚ refl) = <â‚ƒ refl b<c

â‰¤-lublubâ€² : âˆ€ a b c â†’ a â‰¤áµ’ c â†’ b â‰¤áµ’ c â†’ (a âŠ”â‚’ b) â‰¤áµ’ c
â‰¤-lublubâ€² a b c (injâ‚ x) (injâ‚ y) = injâ‚ (<-lublub _ _ _ x y) 
â‰¤-lublubâ€² a b c (injâ‚ x) (injâ‚‚ refl) = injâ‚‚ (sym (âŠ”â‚’-<áµ’ _ _ x))
â‰¤-lublubâ€² a b c (injâ‚‚ refl) (injâ‚ x) = injâ‚‚ (sym (âŠ”â‚’-<áµ’â€² _ _ x))       
â‰¤-lublubâ€² a b c (injâ‚‚ refl) (injâ‚‚ refl) rewrite âŠ”â‚’-idem a = injâ‚‚ refl     